IMLTT/proofs/boundary/BoundaryIsType.lean
@@ -7,10 +7,10 @@ import IMLTT.proofs.admissable.Weakening
 import IMLTT.proofs.admissable.Substitution
 import IMLTT.proofs.boundary.BoundaryIsCtx
 import IMLTT.proofs.boundary.BoundaryHasType
+import IMLTT.proofs.admissable.Contexts
 
 set_option diagnostics true
 set_option maxHeartbeats 1000000
-
 
 theorem boundary_type :
   (∀ {n : Nat} {Γ : Ctx n}, Γ ctx → Γ ctx) ∧
@@ -27,16 +27,16 @@ theorem boundary_type :
       (motive_4 := fun Γ A A' _hAA => IsType Γ A)
       (motive_5 := fun Γ a a' A _haaA => IsType Γ A)
     case HasTypeVar =>
-      intro n Γ A hA ihA
+      intro n Γ A hA _ihA
       apply weakening_type hA hA
     case HasTypePiIntro =>
-      intro n Γ A b B hbB ihbB
+      intro n Γ A b B _hbB ihbB
       apply IsType.pi_form 
       · have hiCA := boundary_ctx_type ihbB
         apply ctx_extr hiCA
       · apply ihbB
     case HasTypeSigmaIntro =>
-      intro n Γ a A b B haA hbB ihaA ihbB
+      intro n Γ a A b B haA _hbB ihaA ihbB
       apply IsType.sigma_form
       · apply ihaA
       · apply substitution_inv_type
@@ -44,82 +44,79 @@ theorem boundary_type :
         · apply ihbB
         · apply haA
     case HasTypeUnitElim =>
-      intro n Γ A a b hA haA hb1 ihA ihaA ihb1
+      intro n Γ A a b hA _haA hb1 _ihA _ihaA _ihb1
       apply substitution_type
       · apply hb1
       · apply hA
     case HasTypeEmptyElim =>
-      intro n Γ A b hA hb0 ihA ihb0
+      intro n Γ A b hA hb0 _ihA _ihb0
       apply substitution_type
       · apply hb0
       · apply hA
     case HasTypePiElim =>
-      intro n Γ f A B a hfPi haA ihfPi ihaA
+      intro n Γ f A B a _hfPi haA ihfPi _ihaA
       apply substitution_type
       · apply haA
       · apply And.right (pi_is_type_inversion ihfPi)
     case HasTypeSigmaElim =>
-      intro n Γ A B p C c hSi hpSi hC hcC ihSi ihpSi ihC ihcC
+      intro n Γ A B p C c _hSi hpSi _hC _hcC _ihSi _ihpSi ihC _ihcC
       apply substitution_type
       · apply hpSi
       · apply ihC
     case HasTypeIdenElim =>
-      intro n Γ A B b a a' p hB hbB hIden hpIden ihB ihbB ihIden ihpIden
-      rw [substitution_zero_n] -- rewrite to substitution_zero x 4subs
-      apply substitution_type
-      · sorry
-      · sorry
+      intro n Γ A B b a a' p _hB _hbB _hIden _hpIden _ihB ihbB _ihIden _ihpIden
+      apply ihbB
     case HasTypeTyConv =>
-      intro n Γ a A B haA hAB ihaA ihAB
-      sorry
+      intro n Γ a A B _haA hAB _ihaA _ihAB
+      apply defeq_is_type' hAB
     case IsEqualTypeIdenFormEq =>
-      intro n Γ a₁ a₂ A a₃ a₄ haaA haaA' ihaaA ihaaA'
+      intro n Γ a₁ a₂ A a₃ a₄ haaA haaA' _ihaaA _ihaaA'
       have haA := boundary_has_type haaA
       have haA' := boundary_has_type haaA'
       apply IsType.iden_form haA haA'
     case IsEqualTypeUnivElimEq =>
-      intro n Γ A A' hAAU hU
+      intro n Γ A A' hAAU _hU
       have hAU := boundary_has_type hAAU
       apply IsType.univ_elim hAU
     case IsEqualTermVarEq =>
-      intro n Γ A hA ihA
+      intro n Γ A hA _ihA
       apply weakening_type hA hA
     case IsEqualTermPiComp =>
-      intro n Γ A b B a hbB haA ihbB ihaA
+      intro n Γ A b B a _hbB haA ihbB _ihaA
       apply substitution_type
       · apply haA
       · apply ihbB
     case IsEqualTermSigmaComp =>
-      intro n Γ a A b B C c haA hbB hC hcC ihaA ihbB ihC ihcC
+      intro n Γ a A b B C c haA hbB hC _hcC _ihaA _ihbB _ihC _ihcC
       apply substitution_type
       · apply HasType.sigma_intro haA hbB
       · apply hC
     case IsEqualTermIdenComp =>
-      intro n Γ A B b a hB hbB haA ihB ihbB ihaA
-      sorry
+      intro n Γ A B b a _hB _hbB _haA _ihB ihbB _ihaA
+      apply ihbB
     case IsEqualTermUnitElimEq =>
-      intro n Γ A A' a a' b b' hAA haaA hbb1 ihAA ihaaA ihb1
+      intro n Γ A A' a a' b b' _hAA _haaA hbb1 ihAA _ihaaA _ihb1
       apply substitution_type
       · apply boundary_has_type hbb1
       · apply ihAA
     case IsEqualTermEmptyElimEq =>
-      intro n Γ A A' b b' hAA hbb0 ihAA ihb0
+      intro n Γ A A' b b' _hAA hbb0 ihAA _ihb0
       apply substitution_type
       · apply boundary_has_type hbb0
       · apply ihAA
     case IsEqualTermPiIntroEq =>
-      intro n Γ A b b' B A' hbbB ihbbB
+      intro n Γ A b b' B _A' _hbbB ihbbB
       apply IsType.pi_form
       · have hiCA := boundary_ctx_type ihbbB
         apply ctx_extr hiCA
       · apply ihbbB
     case IsEqualTermPiElimEq =>
-      intro n Γ f f' A B a a' hffPi haaA ihffPi ihaaA
+      intro n Γ f f' A B a a' _hffPi haaA ihffPi _ihaaA
       apply substitution_type
       · apply boundary_has_type haaA
       · apply And.right (pi_is_type_inversion ihffPi)
     case IsEqualTermSigmaIntroEq =>
-      intro n Γ a a' A b b' B haaA hbbB ihaaA ihbbB
+      intro n Γ a a' A b b' B haaA _hbbB ihaaA ihbbB
       apply IsType.sigma_form
       · apply ihaaA
       · apply substitution_inv_type
@@ -127,18 +124,18 @@ theorem boundary_type :
         · apply ihbbB
         · apply boundary_has_type haaA
     case IsEqualTermSigmaElimEq =>
-      intro n Γ A B A' B' p p' C C' c c' hSiSi hppSi hCC hccC ihSiSi ihppSi ihCC ihccC
+      intro n Γ A B A' B' p p' C C' c c' _hSiSi hppSi _hCC _hccC _ihSiSi _ihppSi ihCC _ihccC
       apply substitution_type
       · apply boundary_has_type hppSi
       · apply ihCC
     case IsEqualTermIdenIntroEq =>
-      intro n Γ A A' a a' hAA haaA ihAA ihaA
+      intro n Γ A A' a a' _hAA haaA _ihAA _ihaA
       have haA := boundary_has_type haaA
       apply IsType.iden_form haA haA
     case IsEqualTermIdenElimEq =>
-      intro n Γ A B B' b b' a₁ a₃ A' a₂ a₄ p p' hBB hbbB hIdId hppId ihBB ihbbB ihIdId ihppId
-      sorry
+      intro n Γ A B B' b b' a₁ a₃ A' a₂ a₄ p p' _hBB _hbbB _hIdId _hppId _ihBB ihbbB _ihIdId _ihppId
+      apply ihbbB
     case IsEqualTermTyConvEq =>
       intro n Γ a b A B habA hAB ihabA ihA
-      sorry
-    any_goals sorry
+      apply defeq_is_type' hAB
+    any_goals aesop
